hax-secret-integers/src/public_integers.rs
@@ -1,4 +1,5 @@
 use crate::traits::*;
+use hax_lib::*;
 
 pub type I8 = i8;
 pub type U8 = u8;
@@ -53,18 +54,26 @@ impl EncodeOps<U8,4> for U32 {
 }
 
 impl<const N: usize, const B:usize> TryEncodeOps<U8, B> for [U32; N] {
+    // #[hax_lib::requires(N <= 65536 / 4)]
+    // #[hax_lib::ensures(|result| if x.len() == N * 4 {result.is_ok()} else {result.is_err()} )] 
     fn try_to_le_bytes(&self) -> Result<[U8;B],()> {
         try_to_le_bytes(self)
     }
+    // #[hax_lib::requires(N <= 65536 / 4)]
+    // #[hax_lib::ensures(|result| if x.len() == N * 4 {result.is_ok()} else {result.is_err()} )] 
     fn try_to_be_bytes(&self) -> Result<[U8;B],()> {
         try_to_be_bytes(self)
     }
 }
 
 impl<const N: usize> TryDecodeOps<U8> for [U32; N] {
+    // #[hax_lib::requires(N <= 65536 / 4)]
+    // #[hax_lib::ensures(|result| if x.len() == N * 4 {result.is_ok()} else {result.is_err()} )] 
     fn try_from_le_bytes(x:&[U8]) -> Result<Self,()> {
         try_from_le_bytes(x)
     }
+    // #[hax_lib::requires(N <= 65536 / 4)]
+    // #[hax_lib::ensures(|result| if x.len() == N * 4 {result.is_ok()} else {result.is_err()} )] 
     fn try_from_be_bytes(x:&[U8]) -> Result<Self,()> {
         try_from_be_bytes(x)
     }
