proof-libs/fstar/core/Core.Array.fst
@@ -8,5 +8,5 @@ let impl_23__map #a n #b (arr: t_Array a n) (f: a -> b): t_Array b n
 
 let impl_23__as_slice #a len (arr: t_Array a len): t_Slice a = arr
 
-let from_fn #a len (f: usize -> a): t_Array a len = admit()
+let from_fn #a len (f: (i:usize{v i < v len}) -> a): t_Array a len = admit()
 
